Capless/Term.lean
@@ -65,10 +65,12 @@ inductive Term : Nat -> Nat -> Nat -> Type where
 | boundary : Classifier -> SType n m k -> Term (n+1) m (k+1) -> Term n m k
 /-- Intercept: `intercept[K] in t` --/
 | intercept : Kind -> Term n m k -> Term n m k
-/-- Unwraps a maybe. --/
-| unwrap : Fin n -> Term n m k
-/-- Unwraps a maybe, but with an additional handler for intercepted labels. --/
-| unwrap_handle : Fin n -> Term (n+2) (m+1) k -> Term n m k
+/-- Unwraps a maybe --/
+| unwrap: Fin n -> Term (n+2) (m+1) k -> Term n m k
+/-- value form of maybe: a returned value -/
+| ok : Fin n -> Term n m k
+/-- value form of maybe: a invocation label, and its associated value. -/
+| invoked : Fin n -> Fin n -> Term n m k
 
 /-!
 ## Notations
@@ -83,7 +85,7 @@ notation:40 "let" "X=" S " in " t => Term.bindt S t
 notation:40 "let" "c=" C " in " t => Term.bindc C t
 notation:40 "boundary[" c "]:" S " in " t => Term.boundary c S t
 notation:40 "intercept[" K "]"" in " t => Term.intercept K t
-notation:40 "handle " n " with " t => Term.unwrap_handle n t
+notation:40 "handle " n " with " t => Term.unwrap n t
 
 /-- Whether this term is a value? -/
 @[aesop safe constructors]
@@ -92,6 +94,8 @@ inductive Term.IsValue : Term n m k -> Prop where
 | tlam : Term.IsValue (tlam S t)
 | clam : Term.IsValue (clam B t)
 | pack : Term.IsValue (pack c x)
+| ok : Term.IsValue (ok v)
+| invoked : Term.IsValue (invoked l v)
 
 /-!
 ## Renaming Operations on `Term`
@@ -115,8 +119,10 @@ def Term.rename (t : Term n m k) (f : FinFun n n') : Term n' m k :=
   | Term.bindc c t => Term.bindc (c.rename f) (t.rename f)
   | Term.boundary c S t => Term.boundary c (S.rename f) (t.rename f.ext)
   | Term.intercept K t => Term.intercept K (t.rename f)
-  | Term.unwrap x => Term.unwrap (f x)
-  | Term.unwrap_handle x t => Term.unwrap_handle (f x) (t.rename f.ext.ext)
+  | Term.unwrap x t => Term.unwrap (f x) (t.rename f.ext.ext)
+  | Term.ok v => Term.ok $ f v
+  | Term.invoked l v => Term.invoked (f l) (f v)
+
 
 def Term.trename (t : Term n m k) (f : FinFun m m') : Term n m' k :=
   match t with
@@ -135,8 +141,9 @@ def Term.trename (t : Term n m k) (f : FinFun m m') : Term n m' k :=
   | Term.bindc c t => Term.bindc c (t.trename f)
   | Term.boundary c S t => Term.boundary c (S.trename f) (t.trename f)
   | Term.intercept K t => Term.intercept K (t.trename f)
-  | Term.unwrap x => Term.unwrap x
-  | Term.unwrap_handle x t => Term.unwrap_handle x (t.trename f.ext)
+  | Term.unwrap x t => Term.unwrap x (t.trename f.ext)
+  | Term.ok v => Term.ok v
+  | Term.invoked l v => Term.invoked l v
 
 def Term.crename (t : Term n m k) (f : FinFun k k') : Term n m k' :=
   match t with
@@ -155,8 +162,9 @@ def Term.crename (t : Term n m k) (f : FinFun k k') : Term n m k' :=
   | Term.bindc c t => Term.bindc (c.crename f) (t.crename f.ext)
   | Term.boundary c S t => Term.boundary c (S.crename f) (t.crename f.ext)
   | Term.intercept K t => Term.intercept K (t.crename f)
-  | Term.unwrap x => Term.unwrap x
-  | Term.unwrap_handle x t => Term.unwrap_handle x (t.crename f)
+  | Term.unwrap x t => Term.unwrap x (t.crename f)
+  | Term.ok v => Term.ok v
+  | Term.invoked l v => Term.invoked l v
 
 def Term.weaken (t : Term n m k) : Term (n+1) m k := t.rename FinFun.weaken
 
@@ -267,10 +275,12 @@ theorem Term.rename_id {t : Term n m k} :
     simp [Term.rename, SType.rename_id, ih, FinFun.id_ext]
   case intercept ih =>
     simp [Term.rename, ih]
-  case unwrap =>
-    simp [Term.rename, FinFun.id]
-  case unwrap_handle ih =>
+  case unwrap ih =>
     simp [Term.rename, FinFun.id_ext, ih, FinFun.id]
+  case ok =>
+    simp [Term.rename, FinFun.id]
+  case invoked =>
+    simp [Term.rename, FinFun.id]
 
 theorem Term.trename_id {t : Term n m k} :
   t.trename FinFun.id = t := by
@@ -310,10 +320,10 @@ theorem Term.trename_id {t : Term n m k} :
     simp [Term.trename, SType.trename_id, ih, FinFun.id_ext]
   case intercept ih =>
     simp [Term.trename, ih]
-  case unwrap =>
-    simp [Term.trename]
-  case unwrap_handle ih =>
+  case unwrap ih =>
     simp [Term.trename, FinFun.id_ext, ih]
+  case ok => simp [Term.trename]
+  case invoked => simp [Term.trename]
 
 theorem Term.crename_id {t : Term n m k} :
   t.crename FinFun.id = t := by
@@ -353,10 +363,10 @@ theorem Term.crename_id {t : Term n m k} :
     simp [ih, SType.crename_id, FinFun.id_ext]
   case intercept ih =>
     simp [Term.crename, ih]
-  case unwrap =>
-    simp [Term.crename]
-  case unwrap_handle ih =>
+  case unwrap ih =>
     simp [Term.crename, ih]
+  case ok => simp [Term.crename]
+  case invoked => simp [Term.crename]
 
 theorem Term.rename_rename {t : Term n m k} {f : FinFun n n'} {g : FinFun n' n''} :
   (t.rename f).rename g = t.rename (g.comp f) := by
@@ -398,11 +408,11 @@ theorem Term.rename_rename {t : Term n m k} {f : FinFun n n'} {g : FinFun n' n''
     simp [<- FinFun.ext_comp_ext, ih]
   case intercept ih =>
     simp [rename, ih]
-  case unwrap =>
-    simp [rename]
-  case unwrap_handle ih =>
+  case unwrap ih =>
     simp [rename]
     simp [<- FinFun.ext_comp_ext, ih]
+  case ok => simp [rename]
+  case invoked => simp [rename]
 
 theorem Term.crename_crename {t : Term n m k} {f : FinFun k k'} {g : FinFun k' k''} :
   (t.crename f).crename g = t.crename (g.comp f) := by
@@ -444,10 +454,10 @@ theorem Term.crename_crename {t : Term n m k} {f : FinFun k k'} {g : FinFun k' k
     simp [<- FinFun.ext_comp_ext, ih]
   case intercept ih =>
     simp [crename, ih]
-  case unwrap =>
-    simp [crename]
-  case unwrap_handle ih =>
+  case unwrap ih =>
     simp [crename, ih]
+  case ok => simp [crename]
+  case invoked => simp [crename]
 
 theorem Term.trename_trename {t : Term n m k} {f : FinFun m m'} {g : FinFun m' m''} :
   (t.trename f).trename g = t.trename (g.comp f) := by
@@ -489,10 +499,10 @@ theorem Term.trename_trename {t : Term n m k} {f : FinFun m m'} {g : FinFun m' m
     simp [<- FinFun.ext_comp_ext, ih]
   case intercept ih =>
     simp [trename, ih]
-  case unwrap =>
-    simp [trename]
-  case unwrap_handle ih =>
+  case unwrap ih =>
     simp [trename]
     simp [<- FinFun.ext_comp_ext, ih]
+  case ok => simp [trename]
+  case invoked => simp [trename]
 
 end Capless
